examples/lpr_checker/array/compilation/proofsARM8/lpr_arrayProofARM8Script.sml
@@ -17,7 +17,9 @@ val check_unsat_io_events_def = new_specification("check_unsat_io_events_def",["
   |> SIMP_RULE bool_ss [SKOLEM_THM,Once(GSYM RIGHT_EXISTS_IMP_THM)]);
 
 val (check_unsat_sem,check_unsat_output) = check_unsat_io_events_def |> SPEC_ALL |> UNDISCH |> SIMP_RULE std_ss [GSYM PULL_EXISTS]|> CONJ_PAIR
-val (check_unsat_not_fail,check_unsat_sem_sing) = MATCH_MP semantics_prog_Terminate_not_Fail check_unsat_sem |> CONJ_PAIR
+val (check_unsat_not_fail,check_unsat_sem_sing) = check_unsat_sem
+  |> SRULE [lpr_array_compiled,ml_progTheory.prog_syntax_ok_semantics]
+  |> MATCH_MP semantics_prog_Terminate_not_Fail |> CONJ_PAIR
 
 val compile_correct_applied =
   MATCH_MP compile_correct (cj 1 lpr_array_compiled)
